Implemented and verified the Encrypted Data Key and Encrypted Data key List functions (#1)

src/EDK.dfy
@@ -18,7 +18,71 @@ module EDK {
     var provider_id: ByteBuf
     var provider_info: ByteBuf
     var ciphertext: ByteBuf
+
+
+    constructor New(provider_id: ByteBuf, provider_info: ByteBuf, ciphertext: ByteBuf)
+    {
+      this.provider_id := provider_id;
+      this.provider_info := provider_info; 
+      this.ciphertext := ciphertext;
+    }
+    
+    /**
+     * Setting all bytes of an EDK to zero when you declare it will make this safe to call even if some buffers are unused.
+     */
+    method EdkClear()
+    requires GoodByteBuf(this.provider_id) && GoodByteBuf(this.provider_info) && GoodByteBuf(this.ciphertext)
+    modifies this.provider_id.a, this.provider_info.a, this.ciphertext.a
+    {
+      ByteBufClear(this.provider_id);
+      ByteBufClear(this.provider_info);
+      ByteBufClear(this.ciphertext);
+    }
   }
+
+  predicate GoodEDKList(edk_list: seq<EncryptedDataKey>)
+  reads edk_list
+  {
+    var num_keys := |edk_list|;
+    forall k :: 0 <= k < num_keys ==> GoodByteBuf(edk_list[k].provider_id) && GoodByteBuf(edk_list[k].provider_info) && 
+    GoodByteBuf(edk_list[k].ciphertext)
+  }
+  /**
+   * Clears all the EDKs in the list.
+   */
+  method EdkListClear(edk_list: seq<EncryptedDataKey>)
+  requires GoodEDKList(edk_list)
+  modifies set i | 0 <= i < |edk_list| :: edk_list[i].provider_id.a
+  modifies set i | 0 <= i < |edk_list| :: edk_list[i].provider_info.a
+  modifies set i | 0 <= i < |edk_list| :: edk_list[i].ciphertext.a
+  {
+    var num_keys := |edk_list|;
+    var key_idx := 0;
+    while key_idx < num_keys
+          invariant 0 <= key_idx
+          decreases num_keys - key_idx
+          
+    {
+      edk_list[key_idx].EdkClear();
+      key_idx := key_idx + 1; 
+    }
+}
+
+  /**
+   * Copies the EDK data in src to dest.
+   */
+   method EdkClone(dest: EncryptedDataKey, src: EncryptedDataKey)
+   requires GoodByteBuf(dest.provider_id) && GoodByteBuf(dest.provider_info) && GoodByteBuf(dest.ciphertext)
+   requires GoodByteBuf(src.provider_id) && GoodByteBuf(src.provider_info) && GoodByteBuf(src.ciphertext)
+   requires dest.provider_id.len <= src.provider_id.len
+   requires dest.provider_info.len <= src.provider_info.len
+   requires dest.ciphertext.len <= src.ciphertext.len
+   modifies dest.provider_id.a, dest.provider_info.a, dest.ciphertext.a 
+   {
+     ByteBufCopyFromByteBuf(dest.provider_id, src.provider_id);
+     ByteBufCopyFromByteBuf(dest.provider_info, src.provider_info);
+     ByteBufCopyFromByteBuf(dest.ciphertext, src.ciphertext);
+   }
 
   // Upon successful parsing, "edk" as non-null and "cur'" has been advanced.
   // Otherwise, returns "edk" as null and "cur' == cur".
